inversion [typing context reductions] -- cases for p:q?l remain

types/typenv.v
@@ -170,19 +170,40 @@ Defined.
 
 #[global] Declare Instance RWCC: Proper (cCong ==> cCong ==> impl) cCong.
 
+Definition update (g: ctx) (p: participant) (a: queue*local): ctx :=
+  match M.find p g with
+    | Some b => M.add p a g 
+    | None   => g
+  end.
+
 Inductive red: ctx -> lab -> ctx -> Prop :=
   | e_recv  : forall p q sigp sigq gam l Tp s s' Tk xs,
               p <> q ->
-              M.mem p gam = false ->
-              M.mem q gam = false ->
               retc xs l = Some (s, Tk) ->
               subsort s' s ->
-              red (M.add p (((q,l,s')::sigp), Tp) (M.add q (sigq, lt_receive p xs) gam)) (lr q p l) (M.add p (sigp, Tp) (M.add q (sigq, Tk) gam))
+              (
+                match M.find p gam with
+                  | Some (sig', T') => qCong sig' ((q,l,s')::sigp) /\ lCong T' Tp
+                  | _               => False 
+                end
+              ) ->
+              (
+                match M.find q gam with
+                  | Some (sig', T') => qCong sig' sigq /\ lCong T' (lt_receive p xs)
+                  | None            => False
+                end
+              ) ->
+              red gam (lr q p l) (M.add p (sigp, Tp) (M.add q (sigq, Tk) gam))
   | e_send  : forall p q sig gam l s Tk xs,
               p <> q ->
-              M.mem p gam = false ->
               retc xs l = Some (s, Tk) ->
-              red (M.add p (sig, lt_send q xs) gam) (ls p q l) ((M.add p ((sig ++ [(q,l,s)]), Tk)) gam)
+              (
+                match M.find p gam with
+                 | Some (sig', T') => qCong sig' sig /\ lCong T' (lt_send q xs)
+                 | _               => False
+                end
+              ) ->
+              red gam (ls p q l) (M.add p ((sig ++ [(q,l,s)]), Tk) gam)
   | e_struct: forall g g1 g' g1' a,
               cCong g g1 ->
               cCong g1' g' ->
@@ -192,19 +213,64 @@ Definition redE l g := exists g', red g l g'.
 
 Notation Path := (coseq (ctx*lab)) (only parsing).
 
-Inductive eventually {A: Type} (F: coseq A -> Prop): coseq A -> Prop :=
-  | evh: forall xs, F xs -> eventually F xs
-  | evc: forall x xs, eventually F xs -> eventually F (cocons x xs).
+Inductive pathRed (R: Path -> Prop): Path -> Prop :=
+  | rpn: pathRed R [||]
+  | rps: forall x, pathRed R [|x|]
+  | rpc: forall x y ys, R (cocons y ys) -> red (fst x) (snd x) (fst y) -> pathRed R (cocons x (cocons y ys)).
 
-Definition eventualyP := @eventually (ctx*lab).
+Lemma mon_pr: monotone1 pathRed.
+Proof. unfold monotone1.
+       intros.
+       induction IN; intros.
+       constructor.
+       constructor.
+       constructor. apply LE, H.
+       apply H0.
+Qed.
+
+Definition pathRedC pt := paco1 (pathRed) bot1 pt. 
+
+Class path: Type :=
+  mkpath
+  {
+    upth: Path;
+    pobl: pathRedC upth
+  }.
+
+Inductive eventually {A: Type} (F: coseq A -> Prop) (R: coseq A -> Prop): coseq A -> Prop :=
+  | evh: forall x xs, F (cocons x xs) -> eventually F R (cocons x xs)
+  | evc: forall x xs, R xs -> eventually F R (cocons x xs).
+
+(* Definition eventualyP := @eventually (ctx*lab). *)
+(* Definition eventualyP pt := @eventually (@upth pt).  *)
+
+Lemma mon_ev: forall {A} (F: coseq A -> Prop), monotone1 (eventually F).
+Proof. unfold monotone1.
+       intros.
+       induction IN; intros.
+       - apply evh. easy.
+       - apply evc, LE, H. 
+Qed.
+
+Definition eventuallyC {A} (F: coseq A -> Prop) p := paco1 (eventually F) bot1 p.
 
 Inductive alwaysG {A: Type} (F: coseq A -> Prop) (R: coseq A -> Prop): coseq A -> Prop :=
   | alwn: F conil -> alwaysG F R conil
   | alwc: forall x xs, F (cocons x xs) -> R xs -> alwaysG F R (cocons x xs).
 
-Definition alwaysP := @alwaysG (ctx*lab).
+(* Definition alwaysP := @alwaysG (ctx*lab).  *)
 
-Definition alwaysC F p := paco1 (alwaysP F) bot1 p.
+(* Definition alwaysP := @alwaysG (path). *)
+
+Lemma mon_alw: forall {A} (F: coseq A -> Prop), monotone1 (alwaysG F).
+Proof. unfold monotone1.
+       intros.
+       induction IN; intros.
+       - apply alwn. easy.
+       - apply alwc. easy. apply LE, H0. 
+Qed.
+
+Definition alwaysC {A} (F: coseq A -> Prop) p := paco1 (alwaysG F) bot1 p.
 
 Definition enabled (F: ctx -> Prop) (pt: Path): Prop :=
   match pt with
@@ -225,10 +291,10 @@ Definition hPS (p q: participant) (l: label) (pt: Path): Prop :=
   end.
 
 Definition fairPath (pt: Path): Prop :=
-  (forall p q l l', enabled (redE (ls p q l)) pt -> eventually (hPS p q l') pt) /\
-  (forall p q l,    enabled (redE (lr q p l)) pt -> eventually (hPR p q l) pt).
+  (forall p q l l', enabled (redE (ls p q l)) pt -> eventuallyC (hPS p q l') pt) /\
+  (forall p q l,    enabled (redE (lr p q l)) pt -> eventuallyC (hPR p q l) pt).
 
-Definition fairPathC := alwaysC fairPath.
+Definition fairPathC (pt: Path) := pathRedC pt /\ alwaysC fairPath pt.
 
 Definition enqueued (p q: participant) (l: label) (s: local.sort) sig (T: local) (pt: Path): Prop :=
   match pt with
@@ -257,35 +323,430 @@ Definition dequeued (p q: participant) (l: label) (s: local.sort) sigp ys (pt: P
   end.
 
 Definition livePath (pt: Path): Prop :=
-  (forall p q l s sig T,  enqueued p q l s sig T pt  -> eventually (hPR q p l) pt) /\
-  (forall p q l s sig ys, dequeued p q l s sig ys pt -> eventually (hPR p q l) pt).
+  (forall p q l s sig T,  enqueued p q l s sig T pt  -> eventuallyC (hPR q p l) pt) /\
+  (forall p q l s sig ys, dequeued p q l s sig ys pt -> eventuallyC (hPR p q l) pt).
 
-Definition livePathC := alwaysC livePath.
+
+Definition livePathC (pt: Path) := pathRedC pt /\ alwaysC livePath pt.
+
+(* Definition livePathC (pt: path) := alwaysC livePath (@upth pt). *)
 
 Definition live (g: ctx) := forall (pt: Path) (l: lab), fairPathC (cocons (g, l) pt) -> livePathC (cocons (g, l) pt).
 
+Require Import Coq.Program.Equality.
+
 Lemma cong_red: forall g g' gr l, red g l gr -> cCong g g' -> red g' l gr.
-Proof. intros. revert g' H0. 
+Proof. intros.
+       revert g' H0.
        induction H; intros.
-       - apply e_struct with (g1  := (M.add p ((q, l, s') :: sigp, Tp) (M.add q (sigq, lt_receive p xs) gam))) 
+       - apply e_struct with (g1  := gam)
                              (g1' := (M.add p (sigp, Tp) (M.add q (sigq, Tk) gam))).
-         rewrite <- H4. easy. easy.
-       - apply e_recv with (s := s); try easy.
-       - eapply e_struct with (g1  := (M.add p (sig, lt_send q xs) gam)) 
+         easy. easy.
+       - apply e_recv with (s := s) (s' := s') (xs := xs); try easy.
+       - eapply e_struct with (g1  := gam) 
                               (g1' := (M.add p (sig ++ [(q, l, s)], Tk) gam)).
          rewrite <- H2. easy. easy.
-         apply e_send; easy.
+         apply e_send with (xs := xs); easy.
        - apply e_struct with (g1 := g) (g1' := g1').
          rewrite H2. easy.
          rewrite H0. easy.
          apply IHred. rewrite H. easy.
 Qed.
 
+Lemma cong_fair: forall g g' l pt,
+  fairPathC (cocons (g,l) pt) ->
+  cCong g g' ->
+  fairPathC (cocons (g',l) pt).
+Proof. (* pcofix CIH. *)
+       intros. destruct H as (Hr,H).
+       pinversion H.
+       subst.
+       split.
+       pinversion Hr. subst.
+       pfold. constructor.
+       subst. simpl in H6. 
+       pfold. constructor. left. easy.
+       simpl. eapply cong_red with (g' := g') in H6; easy.
+       apply mon_pr.
+       pfold. constructor.
+       split. destruct H3 as (H3a,H3b).
+       intros. simpl in H1.
+       destruct H1 as (g'',H1).
+       specialize(H3a p q l0 l').
+       assert(enabled (redE (ls p q l0)) (cocons (g, l) pt)).
+       { simpl. exists g''. apply cong_red with (g := g'). easy. easy. }
+       apply H3a in H2.
 
-Lemma _49: forall g l g', live g -> red g l g' -> live g'.
-Proof. pcofix CIH. intros.
-       pinversion H2.
-       subst. pfold.
-       constructor.
-       unfold live in H0.
-Admitted.
+       pinversion H2. subst. pfold. constructor. easy.
+       subst. pfold. apply evc. left. easy.
+       apply mon_ev.
+
+       intros. simpl in H1.
+       destruct H1 as (g'',H1).
+       destruct H3 as (H3a,H3b).
+       specialize(H3b p q l0).
+       assert(enabled (redE (lr p q l0)) (cocons (g, l) pt)).
+       { simpl. exists g''. apply cong_red with (g := g'). easy. easy. }
+       apply H3b in H2.
+
+       pinversion H2. subst. pfold. constructor. easy.
+       subst. pfold. apply evc. left. easy.
+       apply mon_ev.
+
+       left. easy.
+       apply mon_alw.
+Qed.
+
+Lemma qinvF: forall sig a, qCong nil (a :: sig) -> False. 
+Proof. intro xs.
+       induction xs; intros.
+       - inversion H.
+         assert(q = nil).
+         { case_eq q; intros; subst; easy. }
+         subst. easy.
+         assert(q = nil).
+         { case_eq q; intros; subst; easy. }
+         subst. easy.
+         assert(q1 = nil /\ q2 = nil /\ q3 = nil).
+         { case_eq q1; case_eq q2; case_eq q3; intros; subst; easy. }
+         destruct H0 as (Ha,(Hb,Hc)).
+         subst. easy.
+         assert(q = nil /\ [:: (p1, l1, s1), (p2, l2, s2) & q'] = nil).
+         { case_eq q; intros; subst; easy. }
+         destruct H3 as (Ha,Hb). subst. easy.
+      - inversion H.
+         assert(q = nil).
+         { case_eq q; intros; subst; easy. }
+         subst. easy.
+         assert(q = nil).
+         { case_eq q; intros; subst; easy. }
+         subst. easy.
+         assert(q1 = nil /\ q2 = nil /\ q3 = nil).
+         { case_eq q1; case_eq q2; case_eq q3; intros; subst; easy. }
+         destruct H0 as (Ha,(Hb,Hc)).
+         subst. easy.
+         assert(q = nil /\ [:: (p1, l1, s1), (p2, l2, s2) & q'] = nil).
+         { case_eq q; intros; subst; easy. }
+         destruct H3 as (Ha,Hb). subst. easy.
+Qed.
+
+Lemma qcong_app: forall xs ys a b,
+  qCong xs (b::ys) ->
+  qCong (xs ++ [a]) (b::ys++[a]). 
+Proof. intro xs.
+       induction xs; intros.
+       - apply qinvF in H. easy.
+       - inversion H.
+         rewrite app_nil_r in H1.
+         subst. inversion H1. subst.
+         rewrite app_nil_r.
+         easy.
+         rewrite app_nil_l in H0.
+         subst. inversion H0. subst. easy.
+         rewrite <- app_assoc in H2.
+         rewrite H1 in H2. inversion H2. subst. rewrite H1. easy.
+         rewrite app_comm_cons.
+         rewrite <- H1.
+         assert(((q ++ [:: (p1, l1, s1), (p2, l2, s2) & q']) ++ [a0]) =
+                ((q ++ [(p1, l1, s1)] ++ [(p2, l2, s2)] ++ (q' ++ [a0])))).
+         { simpl. rewrite <- app_assoc. f_equal. }
+         rewrite H3.
+         assert(((q ++ [:: (p2, l2, s2), (p1, l1, s1) & q']) ++ [a0]) =
+                ((q ++ [(p2, l2, s2)] ++ [(p1, l1, s1)] ++ (q' ++ [a0])))).
+         { simpl. rewrite <- app_assoc. f_equal. }
+         rewrite H4.
+         constructor. easy.
+Qed.
+
+Lemma _B_1: forall g g', live g -> cCong g g' -> live g'.
+Proof. intros.
+       unfold live. intros.
+       symmetry in H0.
+       specialize(cong_fair g' g l pt H1 H0); intro Hf.
+       unfold live in H.
+       apply H in Hf.
+       destruct Hf as (Hr, Hf).
+       pinversion Hf.
+       subst. 
+       split. 
+       pinversion Hr. subst. pfold. constructor. subst. pfold. constructor. left. easy.
+       simpl in H7.
+       simpl. eapply cong_red with (g' := g') in H7; easy.
+       apply mon_pr.
+       pfold. constructor.
+       destruct H4 as (H4a,H4b).
+       split.
+
+       intros.
+       specialize(H4a p q l0 s sig T).
+       assert(enqueued p q l0 s sig T (cocons (g, l) pt) ).
+       { simpl. simpl in H2.
+         destruct H0 as (Ha,(Hb,Hc)).
+         case_eq(M.find p g'); intros.
+         destruct p0 as (c1,t1).
+         rewrite H0 in H2.
+         case_eq(M.find p g); intros.
+         destruct p0 as (c2,t2).
+         specialize(Ha p c1 c2 t1 t2 H0 H3).
+         destruct Ha as (Ha1,Ha2).
+         rewrite <- Ha1, <- Ha2. easy.
+         specialize(Hb p c1 t1 H0 H3).
+         destruct Hb as (Hb1,Hb2).
+         destruct H2 as (H2a,H2b).
+         rewrite Hb1 in H2a.
+         apply qinvF in H2a. easy.
+         rewrite H0 in H2.
+         easy.
+       } 
+       apply H4a in H3.
+       pinversion H3. subst. pfold. constructor. easy.
+       subst. pfold. apply evc. left. easy.
+       apply mon_ev.
+       
+       intros.
+       specialize(H4b p q l0 s sig ys).
+       assert(dequeued p q l0 s sig ys (cocons (g, l) pt)).
+       { simpl. simpl in H2.
+         destruct H0 as (Ha,(Hb,Hc)).
+         case_eq(M.find p g'); intros.
+         destruct p0 as (c1,t1).
+         rewrite H0 in H2.
+         case_eq(M.find p g); intros.
+         destruct p0 as (c2,t2).
+         specialize(Ha p c1 c2 t1 t2 H0 H3).
+         destruct Ha as (Ha1,Ha2).
+         rewrite <- Ha1, <- Ha2. easy.
+         specialize(Hb p c1 t1 H0 H3).
+         destruct Hb as (Hb1,Hb2).
+         destruct H2 as (H2a,(H2b,H2c)).
+         rewrite Hb2 in H2c.
+         inversion H2c.
+         rewrite H0 in H2.
+         easy.
+       }
+       apply H4b in H3.
+       pinversion H3. subst. pfold. constructor. easy.
+       subst. pfold. apply evc. left. easy.
+       apply mon_ev.
+
+       left. easy.
+       apply mon_alw.
+Qed.
+
+Lemma ev_or: forall {A: Type} (F: coseq A -> Prop) x xs, 
+  eventuallyC F (cocons x xs) ->
+  F (cocons x xs) \/ eventuallyC F xs.
+Proof. intros.
+       pinversion H.
+       subst. left. easy.
+       subst. right. easy.
+       apply mon_ev.
+Qed.
+
+Lemma red_rcv_inv: forall g g' p r l l',
+  l = lr p r l' -> 
+  red g l g' ->
+  exists ys s t s' sigp,
+  match M.find p g with
+    | Some (que, T) => lCong T (lt_receive r ys) /\ Some (s, t) = retc ys l' /\ p <> r
+    | _             => False
+  end /\
+  match M.find r g with
+    | Some (que, T) => qCong que ((p,l',s')::sigp) /\ subsort s' s /\ p <> r
+    | _             => False
+  end.
+Proof. intros.
+       induction H0; intros.
+       - inversion H. subst.
+         destruct (M.find p gam). destruct p0.
+         exists xs. exists s. exists Tk. exists s'. exists sigp. split. easy.
+         destruct (M.find r gam). destruct p0.
+         easy. easy. easy.
+       - easy.
+         subst.
+         assert(lr p r l' = lr p r l') by easy.
+         specialize(IHred H).
+         destruct IHred as (ys,(s,(t,(s',(sig',(IH1, IH2)))))).
+         exists ys. exists s. exists t. exists s'. exists sig'.
+         case_eq(M.find p g1); intros.
+         + destruct p0 as (c1, t1).
+           rewrite H3 in IH1.
+           destruct IH1 as (Hys,(Hys1,Hys2)).
+           case_eq(M.find p g); intros.
+           ++ destruct p0 as (c2, t2).
+              pose proof H0 as Haa.
+              destruct H0 as (Ha,(Hb,Hc)).
+              specialize(Ha p c2 c1 t2 t1 H4 H3).
+              rewrite <- Hys. split. easy.
+              case_eq(M.find r g1); intros.
+              * destruct p0 as (c3, t3).
+                rewrite H0 in IH2.
+                destruct IH2 as (Hs,Hs1).
+                case_eq(M.find r g); intros.
+                ** destruct p0 as (c4,t4).
+                   destruct Haa as (Haa,(Hab,Hac)).
+                   specialize(Haa r c4 c3 t4 t3 H5 H0).
+                   destruct Haa as (Haa1, Haa2).
+                   rewrite <- Hs. easy.
+                ** destruct Haa as (Haa,(Hab,Hac)).
+                   specialize(Hac r c3 t3 H5 H0).
+                   destruct Hac as (Hac1,Hac2).
+                   rewrite Hac1 in Hs.
+                   apply qinvF in Hs. easy.
+              * rewrite H0 in IH2. easy.
+           ++ destruct H0 as (Ha,(Hb,Hc)).
+              specialize(Hc p c1 t1 H4 H3).
+              rewrite Hys in Hc. easy.
+         + rewrite H3 in IH1. easy.
+Qed.
+
+Lemma red_snd_inv: forall g g' p r l l',
+  l = ls p r l' -> 
+  red g l g' ->
+  exists ys s t,
+  match M.find p g with
+    | Some (que, T) => lCong T (lt_send r ys) /\ Some (s, t) = retc ys l' /\ p <> r
+    | _             => False
+  end.
+Proof. intros.
+       induction H0; intros.
+       - easy.
+       - inversion H. subst.
+         exists xs. exists s. exists Tk.
+         destruct(M.find p gam). destruct p0. easy. easy.
+       - inversion H. subst.
+         assert(ls p r l' = ls p r l') by easy.
+         specialize(IHred H).
+         destruct IHred as (ys, (s, (t, IHred))).
+         exists ys. exists s. exists t.
+         case_eq(M.find p g1); intros.
+         + destruct p0 as (c1, t1).
+           rewrite H4 in IHred.
+           case_eq(M.find p g); intros.
+           ++ destruct p0 as (c2, t2).
+              destruct H0 as (Ha,(Hb,Hc)).
+              specialize(Ha p c2 c1 t2 t1 H5 H4).
+              destruct IHred as (Hys,(Hys1,Hys2)).
+              rewrite <- Hys. easy.
+              destruct H0 as (Ha,(Hb,Hc)).
+              specialize(Hc p c1 t1 H5 H4).
+              destruct Hc as (Hc1,Hc2).
+              destruct IHred as (Hys,(Hys1,Hys2)).
+              rewrite Hc2 in Hys. easy.
+         + rewrite H4 in IHred. easy.
+Qed.
+
+Lemma _B_2_1a: forall g g' g'' p q r l l' l1 l2,
+  l1 = ls p q l ->
+  l2 = lr p r l' ->
+  red g l1 g' -> red g l2 g'' -> False.
+Proof. intros.
+       revert l2 g'' H0 H2.
+       induction H1; intros.
+       - easy.
+       - inversion H. subst.
+         apply red_rcv_inv with (p := p) (r := r) (l' := l') in H4.
+         destruct H4 as (ys,(s1,(t1,(s2,(sigp,(H4a, H4b)))))).
+         destruct( M.find p gam). destruct p0.
+         destruct H4a. rewrite H3 in H2. easy. easy. easy.
+       - subst.
+         apply IHred with (l2 := lr p r l') (g'' := g''). easy. easy.
+         apply cong_red with (g' := g1) in H4; easy.
+Qed.
+
+Lemma _B_2_1b: forall g p q r r' lb1 lb2 l1 l2,
+  p <> r ->
+  lb1 = ls p q l1 -> 
+  lb2 = ls r r' l2 ->
+  (exists g', red g lb2 g') -> (forall g', red g lb1 g' -> exists g'', red g' lb2 g'').
+Proof. intros.
+       induction H3; intros.
+       - easy.
+       - inversion H0. subst.
+         destruct H2 as (g'',H2).
+         apply red_snd_inv with (p := r) (r := r') (l' := l2) in H2.
+         destruct H2 as (ys, (s', (t', H2))).
+         case_eq(M.find r gam); intros.
+         + destruct p0 as (c1, t1).
+           rewrite H1 in H2.
+           exists(M.add r (c1++[(r',l2,s')], t') ((M.add p (sig ++ [(q, l1, s)], Tk) gam))).
+           apply e_send with (xs := ys). easy. easy.
+           rewrite M.add_spec2. rewrite H1. easy.
+           apply String.eqb_neq in H. rewrite H. easy.
+           rewrite H1 in H2. easy.
+           easy.
+       - subst.
+         destruct H2 as (g'', H2).
+         assert(ls p q l1 = ls p q l1 ) by easy.
+         assert((exists g' : ctx, red g1 (ls r r' l2) g') ).
+         { exists g''.
+           apply e_struct with (g1 := g) (g1' := g'').
+           easy. easy. easy.
+         }
+         specialize(IHred H0 H1).
+         destruct IHred as (g''', H3').
+         exists g'''.
+         apply e_struct with (g1 := g1') (g1' := g'''); easy.
+Qed.
+
+Lemma _B_2_1c: forall g p q r r' lb1 lb2 l1 l2,
+  lb1 = ls p q l1 -> 
+  lb2 = lr r r' l2 ->
+  (exists g', red g lb2 g') -> (forall g', red g lb1 g' -> exists g'', red g' lb2 g'').
+Proof. intros.
+       case_eq(String.eqb r p); intros Hneq.
+       rewrite String.eqb_eq in Hneq. subst. 
+       destruct H1.
+       assert((ls p q l1) = (ls p q l1)) by easy.
+       assert(lr p r' l2 = lr p r' l2) by easy.
+       specialize(_B_2_1a g g' x p q r' l1 l2 (ls p q l1) (lr p r' l2) H0 H1 H2 H); intros. easy.
+       induction H2; intros.
+       - easy.
+       - inversion H. subst. 
+         case_eq(M.find p gam); intros.
+         + destruct p0 as (c1, t1).
+           destruct H1 as (g',H1).
+           rewrite H0 in H4.
+           apply red_rcv_inv with (p := r) (r := r') (l' := l2) in H1.
+           destruct H1 as (ys,(s',(t',(s1,(sigp,(H1a, H1b)))))).
+           case_eq(M.find r gam); intros.
+           ++ destruct p0 as (c2, t2).
+              rewrite H1 in H1a.
+              case_eq(String.eqb r' p); intros Heq.
+              rewrite String.eqb_eq in Heq. subst.
+              rewrite H0 in H1b.
+              exists(M.add p ((sigp++[(q, l1, s)]), Tk) (M.add r (c2,t') ((M.add p (sig ++ [(q, l1, s)], Tk) gam)))).
+              apply e_recv with (s := s') (s' := s1) (xs := ys). easy. easy. easy.
+              rewrite M.add_spec1. 
+              destruct H4 as (H4a, H4b). 
+              destruct H1b as (H1b,H1b1).
+              rewrite H4a in H1b.
+              apply qcong_app with (a := (q, l1, s)) in H1b. easy.
+              rewrite M.add_spec2. rewrite H1. easy.
+              rewrite String.eqb_sym. rewrite Hneq. easy.
+              case_eq(M.find r' gam); intros.
+              * destruct p0 as (c3,t3).
+                rewrite H5 in H1b.
+                destruct H1b as (H1b1,(H1b2,H1b3)).
+                exists(M.add r' (sigp, t3) (M.add r (c2,t') ((M.add p (sig ++ [(q, l1, s)], Tk) gam)))).
+                apply e_recv with (s := s') (s' := s1) (xs := ys). easy. easy. easy.
+                rewrite M.add_spec2. rewrite H5. easy.
+                rewrite String.eqb_sym. rewrite Heq. easy.
+                rewrite M.add_spec2. rewrite H1. easy.
+                rewrite String.eqb_sym. rewrite Hneq. easy.
+              * rewrite H5 in H1b. easy.
+           ++ rewrite H1 in H1a. easy. easy.
+         + rewrite H0 in H4. easy.
+       - subst.
+         destruct H1 as (g'', H1).
+         assert(ls p q l1 = ls p q l1 ) by easy.
+         assert((exists g' : ctx, red g1 (lr r r' l2) g') ).
+         { exists g''.
+           apply e_struct with (g1 := g) (g1' := g'').
+           easy. easy. easy.
+         }
+         specialize(IHred H H0).
+         destruct IHred as (g''', H3').
+         exists g'''.
+         apply e_struct with (g1 := g1') (g1' := g'''); easy.
+Qed.
